lot's of different stuff

theories/backtranslations/sem_syn/connective/un_le_syn.v
@@ -1,7 +1,7 @@
 From iris Require Import program_logic.weakestpre.
 From iris.proofmode Require Import tactics.
 From iris_string_ident Require Import ltac2_string_ident.
-From st.prelude Require Import autosubst.
+From st.prelude Require Import autosubst big_op_three.
 From st.lam Require Import types lang typing tactics logrel.definitions logrel.generic.lift.
 From st.lam.lib Require Import fixlam universe.embed_project guard_assert universe.base.
 From st.backtranslations.un_syn Require Import logrel.definitions logrel.un_le_syn.fundamental.
@@ -23,45 +23,6 @@ Section connective_un_le_syn.
 
   Definition ge_Connective (τ : type) (grd emb : val) : iProp Σ :=
     ∀ (v v' : val), (valrel_typed τ v v' -∗ exprel (grd v) (emb v')).
-
-  Fixpoint big_sepL3 {PROP : bi} {A B C}
-      (Φ : A → B → C → PROP) (l1 : list A) (l2 : list B) (l3 : list C) : PROP :=
-    match l1, l2, l3 with
-    | [], [], [] => emp
-    | x1 :: l1, x2 :: l2, x3 :: l3 => Φ x1 x2 x3 ∗ big_sepL3 Φ l1 l2 l3
-    | _, _,_ => False
-    end%I.
-
-  Lemma big_sepL3_lookup {A B C}
-      (Φ : A → B → C → iProp Σ) l1 l2 l3 i x1 x2 x3 :
-    l1 !! i = Some x1 → l2 !! i = Some x2 → l3 !! i = Some x3 →
-    big_sepL3 Φ l1 l2 l3 ⊢ Φ x1 x2 x3.
-  Proof.
-    generalize dependent l3.
-    generalize dependent l2.
-    generalize dependent l1.
-    induction i.
-    - intros l1 l2 l3 H1 H2 H3. iIntros "H".
-      destruct l1 as [|a1 k1]; inversion H1. destruct l2 as [|a2 k2]; inversion H2. destruct l3 as [|a3 k3]; inversion H3.
-      simpl. iDestruct "H" as "[a b]". auto.
-    - intros l1 l2 l3 H1 H2 H3.
-      destruct l1 as [|a1 k1]; inversion H1. destruct l2 as [|a2 k2]; inversion H2. destruct l3 as [|a3 k3]; inversion H3.
-      iIntros "H".
-      iApply (IHi k1 k2 k3 H0 H4 H5).
-      simpl. iDestruct "H" as "[a b]". auto.
-  Qed.
-
-  Lemma big_sepL3_length {A B C}
-      (Φ : A → B → C → iProp Σ) l1 l2 l3 : big_sepL3 Φ l1 l2 l3 ⊢ ⌜ length l1 = length l2 ⌝ ∧ ⌜ length l2 = length l3 ⌝.
-  Proof.
-    generalize dependent l3.
-    generalize dependent l2.
-    generalize dependent l1.
-    induction l1.
-    - intros. destruct l2; destruct l3; auto.
-    - intros. destruct l2; destruct l3; auto.
-      iIntros "H". simpl. rewrite IHl1. iDestruct "H" as "[H %I]". iPureIntro. lia.
-  Qed.
 
   Lemma connective_ep_ga (τ : type) (τs : list type) (pCnτ : Closed_n (length τs) τ) (eps gas : list val) :
     □ (big_sepL3
