theories/backtranslations/sem_syn/connective/syn_le_un.v
@@ -1,0 +1,22 @@
+From iris Require Import program_logic.weakestpre.
+From iris.proofmode Require Import tactics.
+From iris_string_ident Require Import ltac2_string_ident.
+From st.prelude Require Import autosubst.
+From st.lam Require Import types lang typing tactics logrel.definitions logrel.generic.lift.
+From st.lam.lib Require Import fixlam universe.embed_project guard_assert universe.base.
+From st.backtranslations.un_syn Require Import logrel.definitions.
+(* logrel.un_le_syn.fundamental. *)
+
+(* Defines connective lemma between the untyped and typed logic relations (the (syntactically typed ≤ untyped)-refinement) *)
+(* Of the two refinements, this is the easier one *)
+Section connective_syn_le_un.
+
+  Instance rfn' : refinement := syn_le_un.
+
+  Context `{Σ : !gFunctors}.
+  Context `{irisG_inst : !irisG lam_lang Σ}.
+
+
+  Print Instances refinement.
+
+End connective_syn_le_un.
