theories/backtranslations/sem_syn/no_op.v
@@ -1,0 +1,161 @@
+From iris Require Import program_logic.weakestpre.
+From iris.proofmode Require Import tactics.
+From iris_string_ident Require Import ltac2_string_ident.
+From st.prelude Require Import autosubst.
+From st.lam Require Import types lang typing tactics logrel.definitions logrel.generic.lift.
+From st.lam.lib Require Import fixlam universe.embed_project guard_assert universe.base.
+From st.backtranslations.un_syn Require Import logrel.definitions logrel.un_le_syn.fundamental.
+
+(* Note: Proving *)
+(* ∀ (v v' : val), (valrel_typed τ v v') ⊢ (exprel_typed τ v (guard τ v')) *)
+(* does not work out as termination of guard τ v' depends on complete relatedness of valrel_typed τ v v'. *)
+
+Section guard_assert_no_op.
+
+  Context `{Σ : !gFunctors}.
+  Context `{irisG_inst : !irisG lam_lang Σ}.
+
+  Context (s : stuckness).
+
+  Notation valrel_typed := (valrel_typed s).
+  Notation exprel_typed := (exprel_typed s).
+
+  Definition NoOpGuard (τ : type) (grd : val) : iProp Σ :=
+    ∀ (v v' : val), (valrel_typed τ v v') -∗ (exprel_typed τ v (grd v')).
+
+  Definition NoOpAssert (τ : type) (asr : val) : iProp Σ :=
+    ∀ (v v' : val), (valrel_typed τ v v') -∗ (exprel_typed τ v (asr v')).
+
+  Lemma no_op_ga (τ : type) (τs : list type) (pCnτ : Closed_n (length τs) τ) (gas : list val) :
+    □ ([∗ list] τ ; ga ∈ τs ; gas ,
+                            NoOpGuard τ (LamV (Fst (ga.{ren (+1)} ()) %0)) ∧
+                            NoOpAssert τ (LamV (Snd (ga.{ren (+1)} ()) %0)))%Eₙₒ
+      ⊢ NoOpGuard τ.[subst_list τs] (ga_pair Guard τ).{subst_list_val gas} ∧
+    NoOpAssert τ.[subst_list τs] (ga_pair Assert τ).{subst_list_val gas}.
+  Proof.
+    generalize dependent gas.
+    generalize dependent τs.
+    induction τ as [ | | | τ1 IHτ1 τ2 IHτ2 | τ1 IHτ1 τ2 IHτ2 | τ1 IHτ1 τ2 IHτ2 | τb IHτb | X ] ; intros τs pCnτ gas.
+    - admit.
+    - admit.
+    - admit.
+    - admit.
+    - admit.
+    - admit.
+    - specialize (IHτb (τb.[TRec τb.[subst_list τs]/] :: τs)). iIntros "#H".
+      iLöb as "IHlob".
+      iSplit.
+      + rewrite /NoOpGuard. iIntros (v v') "#Hvv'".
+        iEval rewrite /exprel_typed /=. iEval rewrite /lift. 
+
+
+    - (* TArrow *)
+      iIntros "#H".
+      iDestruct (IHτ1 τs ltac:(closed_solver) gas with "H") as "[IHτ1 IHτ2]".
+      iSplit.
+      + iIntros (v v') "#Hvv'". iEval simpl.
+        (* step right side *)
+        iApply lift_step. auto_lam_step. iEval simplify_custom.
+        iEval repeat rewrite -val_subst_valid; asimpl; repeat rewrite val_subst_valid.
+        (* *)
+        repeat assert (∀ e, Lam e = of_val $ LamV e) as ->; auto.
+        iApply lift_val.
+        iEval rewrite valrel_typed_TArrow_unfold.
+        do 2 iModIntro.
+        iIntros (w w') "#Hww'".
+        iSpecialize ("IHτ1" $! w w' with "Hww'").
+        (* step right side *)
+        iApply lift_step. auto_lam_step. iEval simplify_custom.
+        iEval repeat rewrite -val_subst_valid; asimpl; repeat rewrite val_subst_valid.
+        (* ih1 *)
+        iApply (lift_bind _ _ _ [AppRCtx _] [AppRCtx _; AppRCtx _]).
+        iSplitL. iApply "IHτ1"; auto. closed_solver.
+        (*  *)
+        iIntros (x x') "Hxx'". iEval simpl.
+        (*  *)
+        iEval (rewrite valrel_typed_TArrow_unfold) in "Hvv'".
+        iApply (lift_bind _ _ _ [] [AppRCtx _]).
+        iSplitL. by iApply "Hvv'". iIntros (y y') "Hyy'". simpl.
+        iApply IHτ2; auto. closed_solver.
+      + iIntros (v v') "#Hvv'". iEval simpl.
+        (* step right side *)
+        iApply lift_step. auto_lam_step. iEval simplify_custom.
+        iEval repeat rewrite -val_subst_valid; asimpl; repeat rewrite val_subst_valid.
+        (* *)
+        repeat assert (∀ e, Lam e = of_val $ LamV e) as ->; auto.
+        iApply lift_val.
+        iEval rewrite valrel_typed_TArrow_unfold.
+        iModIntro. iIntros (w w') "#Hww'".
+        (* step right side *)
+        iApply lift_step. auto_lam_step. iEval simplify_custom.
+        iEval repeat rewrite -val_subst_valid; asimpl; repeat rewrite val_subst_valid.
+        (* ih1 *)
+        iApply (lift_bind _ _ _ [AppRCtx _] [AppRCtx _; AppRCtx _]).
+        iSplitL. iApply IHτ1; auto. closed_solver.
+        (*  *)
+        iIntros (x x') "Hxx'". iEval simpl.
+        (*  *)
+        iEval (rewrite valrel_typed_TArrow_unfold) in "Hvv'".
+        iApply (lift_bind _ _ _ [] [AppRCtx _]).
+        iSplitL. by iApply "Hvv'". iIntros (y y') "Hyy'". simpl.
+        iApply IHτ2; auto. closed_solver.
+    - (* TRec *)
+      iIntros "#H".
+      iLöb as "IHLob".
+      iSplit.
+      + iIntros (v v') "Hvv'".
+        (* step *)
+        iApply lift_step. auto_lam_step. iEval simplify_custom.
+        rewrite FixArrow_subst.
+        iEval repeat rewrite -val_subst_valid. iEval asimpl.
+        iEval repeat rewrite val_subst_valid.
+        iEval rewrite fixgenTRecga_subst.
+        (* step *)
+        iApply lift_step. auto_lam_step. iEval simplify_custom.
+        rewrite FixArrow_subst.
+        iEval repeat rewrite -val_subst_valid. iEval asimpl.
+        iEval repeat rewrite val_subst_valid.
+        iEval rewrite fixgenTRecga_subst.
+        iEval repeat rewrite val_subst_comp.
+        iEval asimpl.
+        (* fixarrow steps *)
+        iApply lift_rtc_steps. apply rtc_lam_step_ctx with (K := fill [AppLCtx _; FstCtx ; AppLCtx _]); first by apply ectx_lang_ctx. eapply nsteps_rtc. apply FixArrow_eval.
+        iEval simpl.
+        (* step *)
+        iApply lift_step. auto_lam_step. iEval simplify_custom.
+        rewrite FixArrow_subst.
+        iEval repeat rewrite -val_subst_valid. iEval asimpl.
+        iEval repeat rewrite val_subst_valid.
+        iEval rewrite fixgenTRecga_subst.
+        iEval repeat rewrite val_subst_comp.
+        iEval asimpl.
+        (* step *)
+        iApply lift_step. auto_lam_step. iEval simplify_custom.
+        iEval repeat rewrite -val_subst_valid. iEval asimpl.
+        (* step *)
+        iApply lift_step. auto_lam_step. iEval simplify_custom.
+        iEval repeat rewrite val_subst_valid.
+        (* step *)
+        iApply lift_step. auto_lam_step. iEval simplify_custom.
+        (* destruct val rel *)
+        iEval (rewrite valrel_typed_TRec_unfold) in "Hvv'". iDestruct "Hvv'" as (w w') "(-> & -> & #Hww')".
+        iEval repeat rewrite val_subst_valid.
+        (* step *)
+        iApply lift_step. auto_lam_step. iEval simplify_custom.
+        repeat rewrite FixArrow_subst.
+        iEval repeat rewrite val_subst_valid.
+        iEval rewrite fixgenTRecga_subst.
+        iEval repeat rewrite val_subst_comp.
+        iEval asimpl.
+        repeat rewrite FixArrow_subst.
+        iEval repeat rewrite val_subst_valid.
+        iEval rewrite fixgenTRecga_subst.
+        iEval repeat rewrite val_subst_comp.
+        iEval asimpl.
+        (* apply IH *)
+        repeat assert (∀ e, Lam e = of_val $ LamV e) as ->; auto.
+        repeat rewrite subst_list_val_cons.
+
+
+  Admitted.
+
