theories/backtranslations/sem_syn/no_op_not_mod.v
@@ -1,0 +1,150 @@
+(* We can prove weaker version, but it will not be modular...; no meaningful compatibility lemmas *)
+
+From iris Require Import program_logic.weakestpre.
+From iris.proofmode Require Import tactics.
+From iris_string_ident Require Import ltac2_string_ident.
+From st.prelude Require Import autosubst.
+From st.lam Require Import types lang typing tactics logrel.definitions logrel.generic.lift.
+From st.lam.lib Require Import fixlam universe.embed_project guard_assert universe.base.
+From st.backtranslations.un_syn Require Import logrel.definitions logrel.un_le_syn.fundamental.
+
+Section guard_assert_no_opV.
+  Context `{irisG_inst : !irisG lam_lang Σ}.
+
+  Context (s : stuckness).
+
+  Notation valrel_typed := (valrel_typed s).
+  Notation exprel_typed := (exprel_typed s).
+
+  Fixpoint depth (v : val) : nat :=
+    match v with
+    | LamV e => 0
+    | LitV v => 0
+    | PairV v1 v2 => max (depth v1) (depth v2)
+    | InjLV v => depth v
+    | InjRV v => depth v
+    | FoldV v => S (depth v)
+    end.
+
+  Definition NoOpGuard (τ : type) (grd : val) : iProp Σ :=
+    ∀ (v v' : val), (valrel_typed τ v v') -∗ (▷^(depth v) exprel_typed τ v (grd v')).
+
+  Definition NoOpAssert (τ : type) (asr : val) : iProp Σ :=
+    ∀ (v v' : val), (valrel_typed τ v v') -∗ (▷^(depth v) exprel_typed τ v (asr v')).
+
+  Lemma no_op_ga (τ : type) (τs : list type) (pCnτ : Closed_n (length τs) τ) (gas : list val) :
+    □ ([∗ list] τ ; ga ∈ τs ; gas ,
+                            NoOpGuard τ (LamV (Fst (ga.{ren (+1)} ()) %0)) ∧
+                            NoOpAssert τ (LamV (Snd (ga.{ren (+1)} ()) %0)))%Eₙₒ
+      ⊢ NoOpGuard τ.[subst_list τs] (ga_pair Guard τ).{subst_list_val gas} ∧
+    NoOpAssert τ.[subst_list τs] (ga_pair Assert τ).{subst_list_val gas}.
+  Proof.
+    generalize dependent gas.
+    generalize dependent τs.
+    induction τ as [ | | | τ1 IHτ1 τ2 IHτ2 | τ1 IHτ1 τ2 IHτ2 | τ1 IHτ1 τ2 IHτ2 | τb IHτb | X ] ; intros τs pCnτ gas.
+    - admit.
+    - admit.
+    - admit.
+    - admit.
+    - admit.
+    - admit.
+    - (* TRec *)
+      iIntros "#H".
+      iLöb as "IHLob".
+      iSplit.
+      + iIntros (v v') "Hvv'".
+        (* step *)
+        iApply lift_step. auto_lam_step. iEval simplify_custom.
+        rewrite FixArrow_subst.
+        iEval repeat rewrite -val_subst_valid. iEval asimpl.
+        iEval repeat rewrite val_subst_valid.
+        iEval rewrite fixgenTRecga_subst.
+        (* step *)
+        iApply lift_step. auto_lam_step. iEval simplify_custom.
+        rewrite FixArrow_subst.
+        iEval repeat rewrite -val_subst_valid. iEval asimpl.
+        iEval repeat rewrite val_subst_valid.
+        iEval rewrite fixgenTRecga_subst.
+        iEval repeat rewrite val_subst_comp.
+        iEval asimpl.
+        (* fixarrow steps *)
+        iApply lift_rtc_steps. apply rtc_lam_step_ctx with (K := fill [AppLCtx _; FstCtx ; AppLCtx _]); first by apply ectx_lang_ctx. eapply nsteps_rtc. apply FixArrow_eval.
+        iEval simpl.
+        (* step *)
+        iApply lift_step. auto_lam_step. iEval simplify_custom.
+        rewrite FixArrow_subst.
+        iEval repeat rewrite -val_subst_valid. iEval asimpl.
+        iEval repeat rewrite val_subst_valid.
+        iEval rewrite fixgenTRecga_subst.
+        iEval repeat rewrite val_subst_comp.
+        iEval asimpl.
+        (* step *)
+        iApply lift_step. auto_lam_step. iEval simplify_custom.
+        iEval repeat rewrite -val_subst_valid. iEval asimpl.
+        (* step *)
+        iApply lift_step. auto_lam_step. iEval simplify_custom.
+        iEval repeat rewrite val_subst_valid.
+        (* step *)
+        iApply lift_step. auto_lam_step. iEval simplify_custom.
+        (* destruct val rel *)
+        iEval (rewrite valrel_typed_TRec_unfold) in "Hvv'". iDestruct "Hvv'" as (w w') "(-> & -> & #Hww')".
+        iEval repeat rewrite val_subst_valid.
+        (* step *)
+        iApply lift_step. auto_lam_step. iEval simplify_custom.
+        repeat rewrite FixArrow_subst.
+        iEval repeat rewrite val_subst_valid.
+        iEval rewrite fixgenTRecga_subst.
+        iEval repeat rewrite val_subst_comp.
+        iEval asimpl.
+        repeat rewrite FixArrow_subst.
+        iEval repeat rewrite val_subst_valid.
+        iEval rewrite fixgenTRecga_subst.
+        iEval repeat rewrite val_subst_comp.
+        iEval asimpl.
+        (* get lob induction and premisis for induction hyp *)
+        iNext.
+        (* apply IH *)
+        repeat assert (∀ e, Lam e = of_val $ LamV e) as ->; auto.
+        repeat rewrite subst_list_val_cons.
+        iApply (lift_bind _ _ _ [FoldCtx] [FoldCtx]).
+        iSplitL.
+        iApply (IHτb (TRec τb.[up (subst_list τs)] :: τs)); auto. closed_solver. iSplitL; auto.
+        { (* using ilob *)
+          iEval (simpl) in "IHLob".
+          iEval (repeat rewrite FixArrow_subst) in "IHLob".
+          iEval (repeat rewrite val_subst_valid) in "IHLob".
+          iEval (repeat rewrite val_subst_comp) in "IHLob".
+          iEval (rewrite fixgenTRecga_subst) in "IHLob".
+          iEval (asimpl) in "IHLob".
+          iEval (simpl).
+          iEval (repeat rewrite FixArrow_subst).
+          iEval (repeat rewrite val_subst_valid).
+          iEval (rewrite fixgenTRecga_subst).
+          iEval (repeat rewrite val_subst_comp).
+          iEval (asimpl).
+          auto.
+        }
+        by asimpl.
+        (* hmm *)
+        iModIntro.
+        iIntros (x x') "#Hxx'".
+        iEval simpl.
+        change (Fold x) with (of_val (FoldV x)). change (Fold x') with (of_val (FoldV x')).
+        iApply lift_val.
+        iEval rewrite valrel_typed_TRec_unfold.
+        iExists x, x'. repeat iSplit; auto. by asimpl.
+      + admit.
+    - (* TVar *)
+      iIntros "#H".
+      destruct (TVar_subst_list_closed_n_length _ _ pCnτ) as [τ [eq1 ->]].
+      iDestruct (big_sepL2_length with "H") as "%Hl".
+      destruct (gas !! X) as [ga |] eqn:eq2; try by exfalso; (assert (length gas ≤ X); first by apply lookup_ge_None); (assert (X < length τs); first by eapply lookup_lt_Some); lia.
+      iDestruct (big_sepL2_lookup _ _ _ _ _ _ eq1 eq2 with "H") as "[#a #b]".
+      iSplit.
+      + asimpl.
+        change (subst_list_val gas X) with ((ids X).[subst_list_val gas]). rewrite (Var_subst_list_val_lookup _ _ _ eq2).
+        rewrite val_subst_valid. auto.
+      + asimpl.
+        change (subst_list_val gas X) with ((ids X).[subst_list_val gas]). rewrite (Var_subst_list_val_lookup _ _ _ eq2).
+        rewrite val_subst_valid. auto.
+  Admitted.
