theories/lam/lib/guard_assert_approx.v
@@ -1,0 +1,91 @@
+From st.prelude Require Import autosubst.
+From st.lam Require Import types lang typing tactics.
+From st.lam.lib Require Import fixlam omega universe.base.
+
+Inductive action :=
+  | Guard
+  | Assert.
+
+Definition opp_action (act : action) :=
+  match act with
+  | Guard => Assert
+  | Assert => Guard
+  end.
+
+Section guard_assert.
+
+  Local Notation "( x ; y )" := (existT x y) (at level 0, format "( x ;  '/  ' y )").
+
+  Inductive lt_type : type → type → Prop :=
+    | lt_TProd_l τ1 τ2 : lt_type τ1 (TProd τ1 τ2)
+    | lt_TProd_r τ1 τ2 : lt_type τ2 (TProd τ1 τ2)
+    | lt_TSum_l τ1 τ2 : lt_type τ1 (TSum τ1 τ2)
+    | lt_TSum_r τ1 τ2 : lt_type τ2 (TSum τ1 τ2)
+    | lt_TArrow_l τ1 τ2 : lt_type τ1 (TArrow τ1 τ2)
+    | lt_TArrow_r τ1 τ2 : lt_type τ2 (TArrow τ1 τ2)
+    | lt_TRec τb : lt_type τb (TRec τb).
+
+  Require Import FunInd Recdef.
+  From Coq.Wellfounded Require Import Lexicographic_Product Union.
+  From Coq.Relations Require Import Relation_Operators.
+  From Coq.Program Require Import Wf.
+
+  Function ga_pair (nτ : { n : nat & type}) (act : action) {wf (lexprod nat (fun _ => type) lt (fun _ => lt_type)) nτ } : val :=
+    match nτ with
+    | (n;τ) =>
+      match n with
+      | O => LamV (Var 0)
+      | S x => (match τ with
+               | TUnit => match act with
+                         | Guard => LamV %0
+                         | Assert => LamV (Seq %0 ())
+                         end
+               | TBool => match act with
+                         | Guard => LamV %0
+                         | Assert => LamV (If %0 true false)
+                         end
+               | TInt => match act with
+                        | Guard => LamV %0
+                        | Assert => LamV (%0 + 0)
+                        end
+               | TProd τ1 τ2 => LamV (LetIn (Fst %0) (LetIn (Snd %1) ((ga_pair (n;τ1) act).{ren (+3)} %1, (ga_pair (n;τ2) act).{ren (+3)} %0)))
+               | TSum τ1 τ2 => LamV (Case %0 (InjL ((ga_pair (n;τ1) act).{ren (+2)} %0)) (InjR ((ga_pair (n;τ2) act).{ren (+2)} %0)))
+               | TArrow τ1 τ2 => LamV (Lam ((ga_pair (n;τ2) act).{ren (+2)} (%1 ((ga_pair (n;τ1) (opp_action act)).{ren (+2)} %0))))
+               | TRec τb => LamV (Fold (ga_pair (x;τb.[TRec τb/]) act (Unfold %0)))
+               | TVar X => ()%Vₙₒ
+               end)%Eₙₒ
+      end
+    end.
+
+  1-7: by (intros; apply right_lex; simplify_eq; constructor) || (by intros; apply left_lex ; lia).
+  apply wf_lexprod. apply lt_wf. intros _. intro τ. apply Acc_intro. induction τ; try by intros τ' abs; inversion abs.
+  Defined.
+
+  Lemma ga_typed_gen (n : nat) (τ : type) (pCτ : Closed_n 0 τ) (act : action) :
+    ∀ Γ, Γ ⊢ₙₒ (ga_pair (n;τ) act) : (τ ⟶ τ).
+  Proof.
+    generalize dependent act.
+    generalize dependent τ.
+    induction n.
+    - intros τ pCτ act Γ. rewrite ga_pair_equation. by repeat econstructor.
+    - intros τ.
+      induction τ as [ | | | τ1 IHτ1 τ2 IHτ2 | τ1 IHτ1 τ2 IHτ2 | τ1 IHτ1 τ2 IHτ2 | τb IHτb | X ];
+        intros pCτ act; rewrite ga_pair_equation; simpl; try by destruct act; repeat econstructor.
+      + repeat econstructor; fold ga_pair.
+        rewrite -val_subst_valid. apply context_weakening3. apply IHτ1. closed_solver.
+        rewrite -val_subst_valid. apply context_weakening3. apply IHτ2. closed_solver.
+      + repeat econstructor; fold ga_pair.
+        rewrite -val_subst_valid. apply context_weakening2. apply IHτ1. closed_solver.
+        rewrite -val_subst_valid. apply context_weakening2. apply IHτ2. closed_solver.
+      + repeat econstructor; fold ga_pair.
+        rewrite -val_subst_valid. apply context_weakening2. apply IHτ2. closed_solver.
+        rewrite -val_subst_valid. apply context_weakening2. apply IHτ1. closed_solver.
+      + constructor. constructor.
+        apply App_typed with (τ1 := (τb.[TRec τb/])).
+        2: constructor; constructor; by asimpl.
+        simpl in *. apply IHn. admit.
+      + admit.
+  Admitted.
+
+
+End guard_assert.
