theories/prelude/big_op_three.v
@@ -1,0 +1,48 @@
+From iris.base_logic Require Import lib.iprop.
+From iris.proofmode Require Import tactics.
+From iris_string_ident Require Import ltac2_string_ident.
+
+Fixpoint big_sepL3 {PROP : bi} {A B C}
+    (Φ : A → B → C → PROP) (l1 : list A) (l2 : list B) (l3 : list C) : PROP :=
+  match l1, l2, l3 with
+  | [], [], [] => emp
+  | x1 :: l1, x2 :: l2, x3 :: l3 => Φ x1 x2 x3 ∗ big_sepL3 Φ l1 l2 l3
+  | _, _,_ => False
+  end%I.
+
+Section big_sepL3_lemmas.
+
+  Context `{Σ : !gFunctors}.
+
+  Lemma big_sepL3_lookup {A B C}
+      (Φ : A → B → C → iProp Σ) l1 l2 l3 i x1 x2 x3 :
+    l1 !! i = Some x1 → l2 !! i = Some x2 → l3 !! i = Some x3 →
+    big_sepL3 Φ l1 l2 l3 ⊢ Φ x1 x2 x3.
+  Proof.
+    generalize dependent l3.
+    generalize dependent l2.
+    generalize dependent l1.
+    induction i.
+    - intros l1 l2 l3 H1 H2 H3. iIntros "H".
+      destruct l1 as [|a1 k1]; inversion H1. destruct l2 as [|a2 k2]; inversion H2. destruct l3 as [|a3 k3]; inversion H3.
+      simpl. iDestruct "H" as "[a b]". auto.
+    - intros l1 l2 l3 H1 H2 H3.
+      destruct l1 as [|a1 k1]; inversion H1. destruct l2 as [|a2 k2]; inversion H2. destruct l3 as [|a3 k3]; inversion H3.
+      iIntros "H".
+      iApply (IHi k1 k2 k3 H0 H4 H5).
+      simpl. iDestruct "H" as "[a b]". auto.
+  Qed.
+
+  Lemma big_sepL3_length {A B C}
+      (Φ : A → B → C → iProp Σ) l1 l2 l3 : big_sepL3 Φ l1 l2 l3 ⊢ ⌜ length l1 = length l2 ⌝ ∧ ⌜ length l2 = length l3 ⌝.
+  Proof.
+    generalize dependent l3.
+    generalize dependent l2.
+    generalize dependent l1.
+    induction l1.
+    - intros. destruct l2; destruct l3; auto.
+    - intros. destruct l2; destruct l3; auto.
+      iIntros "H". simpl. rewrite IHl1. iDestruct "H" as "[H %I]". iPureIntro. lia.
+  Qed.
+
+End big_sepL3_lemmas.
